James C - partially completed chapter 36

isabelle/Chapter36_1_Language.thy
@@ -9,7 +9,7 @@ datatype type =
 | Prod type type
 | Void
 | Sum type type
-| Command
+| Command type
 
 datatype expr = 
   Var var
@@ -36,6 +36,7 @@ and cmnd =
 | Set var expr
 
 primrec insert :: "var => expr => expr"
+    and insert_cmd :: "var => cmnd => cmnd"
 where "insert n (Var v) = Var (incr n v)"
     | "insert n Zero = Zero"
     | "insert n (Suc e) = Suc (insert n e)"
@@ -53,8 +54,15 @@ where "insert n (Var v) = Var (incr n v)"
     | "insert n (InL t1 t2 e) = InL t1 t2 (insert n e)"
     | "insert n (InR t1 t2 e) = InR t1 t2 (insert n e)"
     | "insert n (Fix t e) = Fix t (insert (next n) e)"
+    | "insert n (Cmd c) = Cmd (insert_cmd n c)"
+    | "insert_cmd n (Return e) = Return (insert n e)"
+    | "insert_cmd n (Bind e c) = Bind (insert n e) (insert_cmd (next n) c)"
+    | "insert_cmd n (Declare e c) = Declare (insert n e) (insert_cmd n c)"
+    | "insert_cmd n (Get v) = Get v"
+    | "insert_cmd n (Set v e) = Set v (insert n e)"
 
 primrec remove :: "var => expr => expr"
+    and remove_cmd :: "var => cmnd => cmnd"
 where "remove n (Var v) = Var (subr n v)"
     | "remove n Zero = Zero"
     | "remove n (Suc e) = Suc (remove n e)"
@@ -72,8 +80,15 @@ where "remove n (Var v) = Var (subr n v)"
     | "remove n (InL t1 t2 e) = InL t1 t2 (remove n e)"
     | "remove n (InR t1 t2 e) = InR t1 t2 (remove n e)"
     | "remove n (Fix t e) = Fix t (remove (next n) e)"
+    | "remove n (Cmd c) = Cmd (remove_cmd n c)"
+    | "remove_cmd n (Return e) = Return (remove n e)"
+    | "remove_cmd n (Bind e c) = Bind (remove n e) (remove_cmd (next n) c)"
+    | "remove_cmd n (Declare e c) = Declare (remove n e) (remove_cmd n c)"
+    | "remove_cmd n (Get v) = Get v"
+    | "remove_cmd n (Set v e) = Set v (remove n e)"
 
 primrec subst' :: "var => expr => expr => expr"
+    and subst_cmd' :: "var => expr => cmnd => cmnd"
 where "subst' n e' (Var v) = (if v = n then e' else Var v)"
     | "subst' n e' Zero = Zero"
     | "subst' n e' (Suc e) = Suc (subst' n e' e)"
@@ -93,16 +108,33 @@ where "subst' n e' (Var v) = (if v = n then e' else Var v)"
     | "subst' n e' (InL t1 t2 e) = InL t1 t2 (subst' n e' e)"
     | "subst' n e' (InR t1 t2 e) = InR t1 t2 (subst' n e' e)"
     | "subst' n e' (Fix t e) = Fix t (subst' (next n) (insert first e') e)"
+    | "subst' n e' (Cmd c) = Cmd (subst_cmd' n e' c)"
+    | "subst_cmd' n e' (Return e) = Return (subst' n e' e)"
+    | "subst_cmd' n e' (Bind e c) = Bind (subst' n e' e) (subst_cmd' (next n) (insert first e') c)"
+    | "subst_cmd' n e' (Declare e c) = Declare (subst' n e' e) (subst_cmd' n e' c)"
+    | "subst_cmd' n e' (Get v) = Get v"
+    | "subst_cmd' n e' (Set v e) = Set v (subst' n e' e)"
 
 definition subst :: "expr => expr => expr"
 where "subst e' e = remove first (subst' first (insert first e') e)"
 
+definition subst_cmd :: "expr => cmnd => cmnd"
+where "subst_cmd e' c = remove_cmd first (subst_cmd' first (insert first e') c)"
+
 lemma [simp]: "remove n (insert n e) = e"
-by (induction e arbitrary: n, simp_all)
-sorry
+  and [simp]: "remove_cmd n (insert_cmd n c) = c"
+by (induction e and c arbitrary: n and n, simp_all)
 
 lemma [simp]: "canswap m n ==> insert m (insert n e) = insert (next n) (insert m e)"
-by (induction e arbitrary: n m, simp_all)
-sorry
+  and [simp]: "canswap m n ==> insert_cmd m (insert_cmd n c) = insert_cmd (next n) (insert_cmd m c)"
+by (induction e and c arbitrary: n m and n m, simp_all)
+
+lemma [simp]: "canswap m n ==> insert m (remove n e) = remove (next n) (insert m e)"
+  and [simp]: "canswap m n ==> insert_cmd m (remove_cmd n c) = remove_cmd (next n) (insert_cmd m c)"
+by (induction e and c arbitrary: n m and n m, simp_all)
+
+lemma [simp]: "canswap m n ==> insert m (subst' n e' e) = subst' (next n) (insert m e') (insert m e)"
+  and [simp]: "canswap m n ==> insert_cmd m (subst_cmd' n e' c) = subst_cmd' (next n) (insert m e') (insert_cmd m c)"
+by (induction e and c arbitrary: n m e' and n m e', simp_all)
 
 end
