isabelle/Chapter36_2_Typechecking.thy
@@ -2,53 +2,155 @@ theory Chapter36_2_Typechecking
 imports Chapter36_1_Language
 begin
 
-inductive typecheck :: "type env => expr => type => bool"
-where tc_var [simp]: "lookup gam x = Some t ==> typecheck gam (Var x) t"
-    | tc_zero [simp]: "typecheck gam Zero Nat"
-    | tc_suc [simp]: "typecheck gam e Nat ==> typecheck gam (Suc e) Nat"
-    | tc_isz [simp]: "typecheck gam et Nat ==> typecheck gam e0 t ==> 
-                typecheck (extend gam Nat) es t ==> typecheck gam (IsZ et e0 es) t"
-    | tc_lam [simp]: "typecheck (extend gam t1) e t2 ==> typecheck gam (Lam t1 e) (Arrow t1 t2)"
-    | tc_appl [simp]: "typecheck gam e1 (Arrow t2 t) ==> typecheck gam e2 t2 ==> 
-                typecheck gam (Appl e1 e2) t"
-    | tc_triv [simp]: "typecheck gam Triv Unit"
-    | tc_pair [simp]: "typecheck gam e1 t1 ==> typecheck gam e2 t2 ==> 
-                typecheck gam (Pair e1 e2) (Prod t1 t2)"
-    | tc_projl [simp]: "typecheck gam e (Prod t1 t2) ==> typecheck gam (ProjL e) t1"
-    | tc_projr [simp]: "typecheck gam e (Prod t1 t2) ==> typecheck gam (ProjR e) t2"
-    | tc_abort [simp]: "typecheck gam e Void ==> typecheck gam (Abort t e) t"
-    | tc_case [simp]: "typecheck gam et (Sum t1 t2) ==> typecheck (extend gam t1) el t ==> 
-                typecheck (extend gam t2) er t ==> typecheck gam (Case et el er) t"
-    | tc_inl [simp]: "typecheck gam e t1 ==> typecheck gam (InL t1 t2 e) (Sum t1 t2)"
-    | tc_inr [simp]: "typecheck gam e t2 ==> typecheck gam (InR t1 t2 e) (Sum t1 t2)"
-    | tc_fix [simp]: "typecheck (extend gam t) e t ==> typecheck gam (Fix t e) t"
+primrec is_mobile :: "type => bool"
+where "is_mobile Nat = True"
+    | "is_mobile (Arrow t1 t2) = False"
+    | "is_mobile Unit = True"
+    | "is_mobile (Prod t1 t2) = (is_mobile t1 & is_mobile t2)"
+    | "is_mobile Void = True"
+    | "is_mobile (Sum t1 t2) = (is_mobile t1 & is_mobile t2)"
+    | "is_mobile (Command t) = False"
 
-inductive_cases [elim!]: "typecheck gam (Var x) t"
-inductive_cases [elim!]: "typecheck gam Zero t"
-inductive_cases [elim!]: "typecheck gam (Suc e) t"
-inductive_cases [elim!]: "typecheck gam (IsZ et e0 es) t"
-inductive_cases [elim!]: "typecheck gam (Lam t1 e) t"
-inductive_cases [elim!]: "typecheck gam (Appl e1 e2) t"
-inductive_cases [elim!]: "typecheck gam Triv t"
-inductive_cases [elim!]: "typecheck gam (Pair e1 e2) t"
-inductive_cases [elim!]: "typecheck gam (ProjL e) t"
-inductive_cases [elim!]: "typecheck gam (ProjR e) t"
-inductive_cases [elim!]: "typecheck gam (Abort t1 e) t"
-inductive_cases [elim!]: "typecheck gam (Case et el er) t"
-inductive_cases [elim!]: "typecheck gam (InL t1 t2 e) t"
-inductive_cases [elim!]: "typecheck gam (InR t1 t2 e) t"
-inductive_cases [elim!]: "typecheck gam (Fix t1 e) t"
+inductive typecheck :: "type env => type env => expr => type => bool"
+      and typecheck_cmd :: "type env => type env => cmnd => type => bool"
+where tc_var [simp]: "lookup gam x = Some t ==> typecheck gam sig (Var x) t"
+    | tc_zero [simp]: "typecheck gam sig Zero Nat"
+    | tc_suc [simp]: "typecheck gam sig e Nat ==> typecheck gam sig (Suc e) Nat"
+    | tc_isz [simp]: "typecheck gam sig et Nat ==> typecheck gam sig e0 t ==> 
+                typecheck (extend gam Nat) sig es t ==> typecheck gam sig (IsZ et e0 es) t"
+    | tc_lam [simp]: "typecheck (extend gam t1) sig e t2 ==> 
+                typecheck gam sig (Lam t1 e) (Arrow t1 t2)"
+    | tc_appl [simp]: "typecheck gam sig e1 (Arrow t2 t) ==> typecheck gam sig e2 t2 ==> 
+                typecheck gam sig (Appl e1 e2) t"
+    | tc_triv [simp]: "typecheck gam sig Triv Unit"
+    | tc_pair [simp]: "typecheck gam sig e1 t1 ==> typecheck gam sig e2 t2 ==> 
+                typecheck gam sig (Pair e1 e2) (Prod t1 t2)"
+    | tc_projl [simp]: "typecheck gam sig e (Prod t1 t2) ==> typecheck gam sig (ProjL e) t1"
+    | tc_projr [simp]: "typecheck gam sig e (Prod t1 t2) ==> typecheck gam sig (ProjR e) t2"
+    | tc_abort [simp]: "typecheck gam sig e Void ==> typecheck gam sig (Abort t e) t"
+    | tc_case [simp]: "typecheck gam sig et (Sum t1 t2) ==> typecheck (extend gam t1) sig el t ==> 
+                typecheck (extend gam t2) sig er t ==> typecheck gam sig (Case et el er) t"
+    | tc_inl [simp]: "typecheck gam sig e t1 ==> typecheck gam sig (InL t1 t2 e) (Sum t1 t2)"
+    | tc_inr [simp]: "typecheck gam sig e t2 ==> typecheck gam sig (InR t1 t2 e) (Sum t1 t2)"
+    | tc_fix [simp]: "typecheck (extend gam t) sig e t ==> typecheck gam sig (Fix t e) t"
+    | tc_cmd [simp]: "typecheck_cmd gam sig c t ==> typecheck gam sig (Cmd c) (Command t)"
+    | tc_retn [simp]: "is_mobile t ==> typecheck gam sig e t ==> typecheck_cmd gam sig (Return e) t"
+    | tc_bind [simp]: "typecheck gam sig e (Command t) ==> typecheck_cmd (extend gam t) sig c t' ==> 
+                typecheck_cmd gam sig (Bind e c) t'"
+    | tc_decl [simp]: "is_mobile t ==> typecheck gam sig e t ==> 
+                typecheck_cmd gam (extend sig t) c t' ==>  typecheck_cmd gam sig (Declare e c) t'"
+    | tc_get [simp]: "lookup sig v = Some t ==> typecheck_cmd gam sig (Get v) t"
+    | tc_set [simp]: "lookup sig v = Some t ==> typecheck gam sig e t ==> 
+                typecheck_cmd gam sig (Set v e) t"
 
-lemma [simp]: "typecheck gam e t ==> n in gam ==> 
-         typecheck (extend_at n gam t') (insert n e) t"
-by (induction gam e t arbitrary: n rule: typecheck.induct, fastforce+)
+inductive_cases [elim!]: "typecheck gam sig (Var x) t"
+inductive_cases [elim!]: "typecheck gam sig Zero t"
+inductive_cases [elim!]: "typecheck gam sig (Suc e) t"
+inductive_cases [elim!]: "typecheck gam sig (IsZ et e0 es) t"
+inductive_cases [elim!]: "typecheck gam sig (Lam t1 e) t"
+inductive_cases [elim!]: "typecheck gam sig (Appl e1 e2) t"
+inductive_cases [elim!]: "typecheck gam sig Triv t"
+inductive_cases [elim!]: "typecheck gam sig (Pair e1 e2) t"
+inductive_cases [elim!]: "typecheck gam sig (ProjL e) t"
+inductive_cases [elim!]: "typecheck gam sig (ProjR e) t"
+inductive_cases [elim!]: "typecheck gam sig (Abort t1 e) t"
+inductive_cases [elim!]: "typecheck gam sig (Case et el er) t"
+inductive_cases [elim!]: "typecheck gam sig (InL t1 t2 e) t"
+inductive_cases [elim!]: "typecheck gam sig (InR t1 t2 e) t"
+inductive_cases [elim!]: "typecheck gam sig (Fix t1 e) t"
+inductive_cases [elim!]: "typecheck gam sig (Cmd c) t"
+inductive_cases [elim!]: "typecheck_cmd gam sig (Return e) t"
+inductive_cases [elim!]: "typecheck_cmd gam sig (Bind e c) t"
+inductive_cases [elim!]: "typecheck_cmd gam sig (Declare e c) t"
+inductive_cases [elim!]: "typecheck_cmd gam sig (Get v) t"
+inductive_cases [elim!]: "typecheck_cmd gam sig (Set v e) t"
 
-lemma [simp]: "typecheck (extend_at n gam t') e t ==> n in gam ==> typecheck gam e' t' ==> 
-        typecheck gam (remove n (subst' n (insert n e') e)) t"
-by (induction "extend_at n gam t'" e t arbitrary: n gam t' e' rule: typecheck.induct, fastforce+)
+(*
+lemma [simp]: "typecheck gam sig e t ==> typecheck gam (next sig) e t"
+  and [simp]: "typecheck_cmd gam sig c t ==> typecheck_cmd gam (next sig) c t"
+by (induction rule: typecheck_typecheck_cmd.inducts, simp_all)
+*)
 
-lemma [simp]: "typecheck (extend gam t') e t ==> typecheck gam e' t' ==> 
-                          typecheck gam (subst e' e) t"
+lemma [simp]: "typecheck gam sig e t ==> n in gam ==> 
+         typecheck (extend_at n gam t') sig (insert n e) t"
+  and [simp]: "typecheck_cmd gam sig c t ==> n in gam ==> 
+         typecheck_cmd (extend_at n gam t') sig (insert_cmd n c) t"
+by (induction arbitrary: n and n rule: typecheck_typecheck_cmd.inducts, fastforce+)
+
+lemma [simp]: "typecheck (extend_at n gam t') sig e t ==> n in gam ==> typecheck gam sig e' t' ==> 
+        typecheck gam sig (remove n (subst' n (insert n e') e)) t"
+  and [simp]: "typecheck_cmd (extend_at n gam t') sig c t ==> n in gam ==> 
+        typecheck gam sig e' t' ==> 
+                typecheck_cmd gam sig (remove_cmd n (subst_cmd' n (insert n e') c)) t"
+proof (induction "extend_at n gam t'" sig e t and "extend_at n gam t'" sig c t
+       arbitrary: n gam t' e' and n gam t' e' rule: typecheck_typecheck_cmd.inducts)
+case tc_var
+  thus ?case by fastforce
+next case tc_zero
+  thus ?case by fastforce
+next case tc_suc
+  thus ?case by fastforce
+next case tc_isz
+  thus ?case by fastforce
+next case tc_lam
+  thus ?case by fastforce
+next case tc_appl
+  thus ?case by fastforce
+next case tc_triv
+  thus ?case by fastforce
+next case tc_pair
+  thus ?case by fastforce
+next case tc_projl
+  thus ?case by fastforce
+next case tc_projr
+  thus ?case by fastforce
+next case tc_abort
+  thus ?case by fastforce
+next case tc_case
+  thus ?case by fastforce
+next case tc_inl
+  thus ?case by fastforce
+next case tc_inr
+  thus ?case by fastforce
+next case tc_fix
+  thus ?case by fastforce
+next case tc_cmd
+  thus ?case by fastforce
+next case tc_retn
+  thus ?case by fastforce
+next case tc_bind
+  thus ?case by fastforce
+next case (tc_decl t sig e c t'')
+  from tc_decl have "is_mobile t" by simp
+  from tc_decl have "typecheck (extend_at n gam t') sig e t" by simp
+  from tc_decl have "extend_at n gam t' = extend_at nn ggam tt' \<Longrightarrow>
+  nn in ggam \<Longrightarrow>
+  typecheck ggam sig ee' tt' \<Longrightarrow>
+  typecheck ggam sig (remove nn (subst' nn (insert nn ee') e)) t" by simp
+  from tc_decl have "typecheck_cmd (extend_at n gam t') (extend sig t) c t''" by simp
+  from tc_decl have "extend_at n gam t' = extend_at nn ggam tt' \<Longrightarrow>
+  nn in ggam \<Longrightarrow>
+  typecheck ggam (extend sig t) ee' tt' \<Longrightarrow>
+  typecheck_cmd ggam (extend sig t)
+   (remove_cmd nn (subst_cmd' nn (insert nn ee') c)) t''" by simp
+  from tc_decl have "n in gam" by simp
+  from tc_decl have "typecheck gam sig e' t'" by simp
+
+
+  have "typecheck_cmd gam sig (remove_cmd n (subst_cmd' n (insert n e') (Declare e c))) t''" by simp sorry
+  thus ?case by simp
+next case tc_get
+  thus ?case by fastforce
+next case tc_set
+  thus ?case by fastforce
+qed 
+
+lemma [simp]: "typecheck (extend gam t') sig e t ==> typecheck gam sig e' t' ==> 
+                          typecheck gam sig (subst e' e) t"
 by (simp add: subst_def)
+
+lemma [simp]: "typecheck_cmd (extend gam t') sig c t ==> typecheck gam sig e' t' ==> 
+                          typecheck_cmd gam sig (subst_cmd e' c) t"
+by (simp add: subst_cmd_def)
 
 end
